src/sequential/LowerMemory.v
@@ -108,33 +108,9 @@ Variant lower_event: forall (e_src e_tgt: ThreadEvent.t), Prop :=
 .
 Hint Constructors lower_event.
 
-Variant lower_op_kind: forall (kind_src kind_tgt: Memory.op_kind), Prop :=
-| lower_op_kind_add
-  :
-    lower_op_kind Memory.op_kind_add Memory.op_kind_add
-| lower_op_kind_split
-    ts msg_src msg_tgt
-    (MSG: Message.le msg_src msg_tgt)
-  :
-    lower_op_kind (Memory.op_kind_split ts msg_src) (Memory.op_kind_split ts msg_tgt)
-| lower_op_kind_lower
-    msg_src msg_tgt
-    (MSG: Message.le msg_src msg_tgt)
-  :
-    lower_op_kind (Memory.op_kind_lower msg_src) (Memory.op_kind_lower msg_tgt)
-| lower_op_kind_cancel
-  :
-    lower_op_kind Memory.op_kind_cancel Memory.op_kind_cancel
-.
-Hint Constructors lower_op_kind.
-
 
 Global Program Instance lower_event_PreOrder: PreOrder lower_event.
 Next Obligation. ii. destruct x; try (econs; eauto); refl. Qed.
-Next Obligation. ii. inv H; inv H0; econs; eauto; etrans; eauto. Qed.
-
-Global Program Instance lower_op_kind_PreOrder: PreOrder lower_op_kind.
-Next Obligation. ii. destruct x; econs; eauto; refl. Qed.
 Next Obligation. ii. inv H; inv H0; econs; eauto; etrans; eauto. Qed.
 
 Lemma lower_event_program_event
@@ -407,7 +383,7 @@ Lemma lower_memory_write mem_src0 mem_tgt0
     exists mem_src1 kind_src,
       (<<WRITESRC: Memory.write prom0 mem_src0 loc from to msg_src prom1 mem_src1 kind_src>>) /\
       (<<MEM: lower_memory mem_src1 mem_tgt1>>) /\
-      (<<KIND: lower_op_kind kind_src kind_tgt>>).
+      (<<KIND: kind_src = kind_tgt>>).
 Proof.
   inv WRITETGT. inv PROMISE.
   { hexploit lower_memory_add; eauto. i. des.
@@ -443,7 +419,7 @@ Proof.
       }
     }
     { eapply lower_memory_split; eauto. }
-    { econs; eauto. refl. }
+    { ss. }
   }
   { hexploit lower_succeed_wf; try apply PROMISES; eauto. i. des.
     hexploit (@Memory.lower_exists prom0 loc from to msg0 msg_src); eauto.
@@ -465,7 +441,7 @@ Proof.
       }
     }
     { eapply lower_memory_lower; eauto. }
-    { econs; eauto. refl. }
+    { ss. }
   }
   { inv MSG. hexploit (@Memory.remove_exists_le prom0 mem_src0); eauto. i. des.
     esplits.
@@ -489,8 +465,8 @@ Lemma lower_memory_write_na
     exists mem_src1 kinds_src kind_src,
       (<<WRITESRC: Memory.write_na ts_src prom0 mem_src0 loc from to val prom1 mem_src1 msgs kinds_src kind_src>>) /\
       (<<MEM: lower_memory mem_src1 mem_tgt1>>) /\
-      (<<KINDS: List.Forall2 lower_op_kind kinds_src kinds_tgt>>) /\
-      (<<KIND: lower_op_kind kind_src kind_tgt>>).
+      (<<KINDS: kinds_src = kinds_tgt>>) /\
+      (<<KIND: kind_src = kind_tgt>>).
 Proof.
   revert mem_src0 ts_src TS MEM MLE. induction WRITETGT.
   { i. hexploit lower_memory_write;
@@ -507,8 +483,11 @@ Proof.
     { refl. }
     { eauto. }
     { eapply write_memory_le; eauto. }
-    i. des. esplits; eauto.
-    econs 2; eauto. eapply TimeFacts.le_lt_lt; eauto.
+    i. des. esplits.
+    { econs 2; eauto. eapply TimeFacts.le_lt_lt; eauto. }
+    { eauto. }
+    { f_equal; eauto. }
+    { eauto. }
   }
 Qed.
 
@@ -594,7 +573,7 @@ Lemma lower_memory_write_step mem_src0 mem_tgt0
       (<<LOCAL: lower_local lc_src1 lc_tgt1>>) /\
       (<<RELEASEDW: View.opt_le releasedw_src releasedw_tgt>>) /\
       (<<SC: TimeMap.le sc_src1 sc_tgt1>>) /\
-      (<<KIND: lower_op_kind kind_src kind_tgt>>)
+      (<<KIND: kind_src = kind_tgt>>)
 .
 Proof.
   inv LOCAL. inv STEP.
@@ -641,8 +620,8 @@ Lemma lower_memory_write_na_step
       (<<MEM: lower_memory mem_src1 mem_tgt1>>) /\
       (<<LOCAL: lower_local lc_src1 lc_tgt1>>) /\
       (<<SC: TimeMap.le sc_src1 sc_tgt1>>) /\
-      (<<KINDS: List.Forall2 lower_op_kind kinds_src kinds_tgt>>) /\
-      (<<KIND: lower_op_kind kind_src kind_tgt>>)
+      (<<KINDS: kinds_src = kinds_tgt>>) /\
+      (<<KIND: kind_src = kind_tgt>>)
 .
 Proof.
   inv LOCAL. inv STEP. hexploit lower_memory_write_na; try eassumption.
